src/goose_lang/proofmode.v
@@ -198,13 +198,7 @@ Ltac wp_pure_filter e' :=
   (* For Beta-redices, we do *syntactic* matching only, to avoid unfolding
      definitions. This matches the treatment for [pure_beta] via [AsRecV]. *)
   first [ lazymatch e' with (App (Val (RecV _ _ _)) (Val _)) => idtac end
-        | eunify e' (do: (Val _))%E
-        | eunify e' (return: (Val _))%E
-        | eunify e' (continue: (Val _))%E
-        | eunify e' (break: (Val _))%E
-        | eunify e' (struct.field_ref _ _ (Val _))%E
-        | eunify e' (exception_seq _ (Val _))%E
-        | eunify e' (App exception_do (Val _))%E
+        | pose proof (ltac:(tc_solve) : WpPureExecCandidate e')
         | eunify e' (rec: _ _ := _)%E
         | eunify e' (InjL (Val _))
         | eunify e' (InjR (Val _))
